theories/iris/logrel/compat/case_load_move.v
@@ -1,0 +1,48 @@
+Require Import RecordUpdate.RecordUpdate.
+From stdpp Require Import base list.
+
+From iris.proofmode Require Import base proofmode classes.
+
+From RichWasm.named_props Require Import named_props custom_syntax.
+From RichWasm.wasm Require Import operations.
+From RichWasm Require Import layout syntax typing.
+From RichWasm.compiler Require Import prelude codegen instruction module.
+From RichWasm.iris Require Import autowp memory util wp_codegen.
+From RichWasm.iris.language Require Import cwp logpred.
+From RichWasm.iris.logrel Require Import relations fundamental_kinding.
+
+Set Bullet Behavior "Strict Subproofs".
+Set Default Goal Selector "!".
+
+Section Fundamental.
+
+  Context `{!logrel_na_invs Σ}.
+  Context `{!wasmG Σ}.
+  Context `{!richwasmG Σ}.
+
+  Variable rti : rt_invariant Σ.
+  Variable sr : store_runtime.
+  Variable mr : module_runtime.
+
+  Lemma compat_case_load_move M F L L' wt wt' wtf wl wl' wlf ess es' τs τs' κr κv κs :
+    let fe := fe_of_context F in
+    let WT := wt ++ wt' ++ wtf in
+    let WL := wl ++ wl' ++ wlf in
+    let F' := F <| fc_labels ::= cons (τs', L') |> in
+    let τs_ser := zip_with SerT κs τs in
+    let ψ := InstrT [RefT κr (BaseM MemMM) (VariantT κv τs_ser)] τs' in
+    Forall2
+      (fun τ es =>
+         (forall wt wt' wtf wl wl' wlf es',
+            let fe' := fe_of_context F' in
+            let WT := wt ++ wt' ++ wtf in
+            let WL := wl ++ wl' ++ wlf in
+            run_codegen (compile_instrs mr fe' es) wt wl = inr ((), wt', wl', es') ->
+           ⊢ have_instr_type_sem rti sr mr M F' L WT WL es' (InstrT [τ] τs') L'))
+      τs ess ->
+    has_instruction_type_ok F ψ L' ->
+    run_codegen (compile_instr mr fe (ICaseLoad ψ Move L' ess)) wt wl = inr ((), wt', wl', es') ->
+    ⊢ have_instr_type_sem rti sr mr M F L WT WL es' ψ L'.
+  Admitted.
+
+End Fundamental.
