theories/iris/logrel/compat/load_copy.v
@@ -1,0 +1,837 @@
+From Stdlib Require Import ZArith.
+
+Require Import RecordUpdate.RecordUpdate.
+
+From mathcomp Require Import ssrbool eqtype.
+
+From stdpp Require Import base list.
+
+From iris.proofmode Require Import base proofmode classes.
+
+From RichWasm.named_props Require Import named_props custom_syntax.
+From RichWasm.wasm Require Import operations.
+From RichWasm Require Import layout syntax typing.
+From RichWasm.compiler Require Import prelude codegen instruction module memory.
+From RichWasm.iris Require Import autowp memory util wp_codegen numerics.
+From RichWasm.iris.language Require Import cwp logpred.
+From RichWasm.iris.logrel Require Import relations.
+From RichWasm.iris.logrel.compat Require Import common.
+
+Set Bullet Behavior "Strict Subproofs".
+Set Default Goal Selector "!".
+
+Section Fundamental.
+
+  Context `{!logrel_na_invs Σ}.
+  Context `{!wasmG Σ}.
+  Context `{!richwasmG Σ}.
+
+  Variable rti : rt_invariant Σ.
+  Variable sr : store_runtime.
+  Variable mr : module_runtime.
+
+  Lemma atoms_interp_nil_inv vs :
+    atoms_interp [] vs ⊣⊢ ⌜vs = []⌝ .
+  Proof.
+    iSplit.
+    - setoid_rewrite big_sepL2_nil_inv_l.
+      done.
+    - iIntros (->); cbn; done.
+  Qed.
+
+  Lemma atoms_interp_cons_inv o os vs :
+    ⊢ atoms_interp (o :: os) vs -∗ ∃ v vs', ⌜vs = v :: vs'⌝ ∗ atom_interp o v ∗ atoms_interp os vs'.
+  Proof.
+    iIntros "Hat".
+    iEval (unfold atoms_interp) in "Hat".
+    setoid_rewrite big_sepL2_cons_inv_l.
+    iDestruct "Hat" as (v vs' Hvs) "(Hv & Hvs')".
+    iExists v, vs'; iFrame; done.
+  Qed.
+
+  Lemma atoms_interp_length os vs :
+    ⊢ atoms_interp os vs -∗ ⌜length os = length vs⌝.
+  Proof.
+    iApply big_sepL2_length.
+  Qed.
+
+  Lemma atoms_interp_one_inv o vs :
+    atoms_interp [o] vs ⊣⊢ ∃ v, ⌜vs = [v]⌝ ∗ atom_interp o v.
+  Proof.
+    iSplit.
+    - iIntros "Hvs".
+      iPoseProof (atoms_interp_cons_inv with "Hvs") as (v vs' Heq) "[Hv Hnil]".
+      rewrite atoms_interp_nil_inv.
+      iDestruct "Hnil" as "%Hnil"; subst.
+      iExists v; auto.
+    - iIntros "(%v & -> & Hv)".
+      cbn; auto.
+  Qed.
+
+  Lemma value_interp_ref_sz se κ μ τ os :
+    ⊢ value_interp rti sr se (RefT κ μ τ) (SAtoms os) -∗ ⌜length os = 1⌝.
+  Proof.
+    iIntros "Hv".
+    rewrite value_interp_eq; cbn.
+    iDestruct "Hv" as "(%κ0 & %Heval & Hkind & Hmem)".
+    destruct μ as [| [|]]; auto.
+    - iDestruct "Hmem" as "(%ℓ & %fs & %ws & %Hos & _)".
+      by inversion Hos.
+    - iDestruct "Hmem" as "(%ℓ & %fs & %Hos & _)".
+      by inversion Hos.
+  Qed.
+
+  Lemma rep_ref_kind_ptr F κ μ τ ρ χ δ :
+    has_kind F (RefT κ μ τ) (VALTYPE ρ χ δ) ->
+    ρ = AtomR PtrR /\
+    exists χ', κ = VALTYPE (AtomR PtrR) χ' ExDrop.
+  Proof.
+    intros Hkind.
+    remember (RefT κ μ τ) as ref.
+    remember (VALTYPE ρ χ δ) as val.
+    revert Heqval Heqref.
+    revert ρ χ δ.
+    induction Hkind using has_kind_ind'; intros; try congruence.
+    - subst κ0.
+      split; try congruence.
+      inversion Heqref; eauto.
+    - subst κ0.
+      split; try congruence.
+      inversion Heqref; eauto.
+    - subst κ'.
+      inversion H; subst; eapply IHHkind; eauto.
+  Qed.
+
+  Lemma Z_even_mod_even :
+    forall n k : Z,
+    Z.even k = true ->
+    Z.even (n mod k) = Z.even n.
+  Proof.
+    intros n k Hk.
+    apply Bool.eq_true_iff_eq.
+
+    assert (Hk2 : (k mod 2)%Z = 0).
+    { rewrite Zmod_even. by rewrite Hk. }
+    destruct (Z.eq_dec k 0) as [Hk0 | Hk0].
+    { subst. by rewrite Zmod_0_r. }
+
+    rewrite (Z.mod_eq n k); last done.
+
+    replace (n - k * (n / k))%Z with (n + (k * -(n / k)))%Z; last lia.
+    rewrite Z.even_add_mul_even.
+    2: { rewrite <- Z.even_spec. rewrite Zeven_mod. lia. }
+    done.
+  Qed.
+
+  Lemma Z_Even_mod_Even :
+    forall n k, Z.Even k -> Z.Even (n mod k) <-> Z.Even n.
+  Proof.
+    intros n k Hk.
+    do 2 rewrite <- Z.even_spec.
+    rewrite Z_even_mod_even; first done.
+    by apply Z.even_spec.
+  Qed.
+
+  Lemma Z_mod_even_mod_2 :
+    forall n k,
+    Z.Even k ->
+    ((n mod k) mod 2)%Z = (n mod 2)%Z.
+  Proof.
+    intros n k Hk.
+    rewrite Zmod_even.
+    rewrite Z_even_mod_even; last by rewrite Z.even_spec.
+    symmetry.
+    apply Zmod_even.
+  Qed.
+
+  Lemma mod32_mod2 (n: Z) :
+    (((2 * n) mod 4294967296) mod 2)%Z = 0.
+  Proof.
+    rewrite Z_mod_even_mod_2; last by rewrite <- Z.even_spec.
+    rewrite Zmod_even.
+    by rewrite Z.even_even.
+  Qed.
+
+  Lemma root_pointer_heap_shp_inv rp μ ℓ :
+    root_pointer_interp rp (PtrHeap μ ℓ) -∗
+    ⌜∃ a, rp = RootHeap μ a⌝.
+  Proof.
+    iIntros "H".
+    destruct rp; first done.
+    cbn.
+    iDestruct "H" as "(-> & _)".
+    by iExists _.
+  Qed.
+
+  Lemma wp_load_w μ t off wt wl wt' wl' es ret :
+    run_codegen (load_w mr μ t off) wt wl = inr (ret, wt', wl', es) ->
+    ret = () /\
+    wt' = [] /\
+    wl' = [] /\
+    forall ℓ ℓ32 memidx memidxN (f: frame) B R Φ v,
+        N_i32_repr ℓ ℓ32 ->
+        N_nat_repr memidx memidxN ->
+        inst_memory (f_inst f) !! base_mem_idx mr μ = Some memidx ->
+        types_agree t v ->
+        ⊢ ↪[frame] f -∗
+          ↪[RUN] -∗
+          memidxN ↦[wms][ℓ + byte_offset μ off]bits v -∗
+          ▷ (memidxN↦[wms][ℓ + byte_offset μ off]bits v -∗ Φ f [v]) -∗
+          CWP W.BI_const (VAL_int32 ℓ32) :: es UNDER B; R {{ Φ }}.
+  Proof.
+    intros Hcg.
+    unfold load_w in Hcg.
+    inv_cg_emit Hcg; subst es wt' wl' ret.
+    split; [auto|].
+    split; [auto|].
+    split; [auto|].
+    intros * Hℓ Hmemidx Hmem Hty.
+    iIntros "Hf Hrun Hptr HΦ".
+    iApply (cwp_load with "[$] [$] [$] [$]"); eauto.
+  Qed.
+
+  Lemma wp_mem_load1_copy_mm
+    se fe lidx off ι wt wl ret wt' wl' es fs ws ℓ ℓ32 τ π B R
+    (f: frame) memidx memidxN v Φ :
+    run_codegen (memory.load1 mr fe MemMM Copy lidx off ι) wt wl = inr (ret, wt', wl', es) ->
+    N_i32_repr ℓ ℓ32 ->
+    N_nat_repr memidx memidxN ->
+    inst_memory (f_inst f) !! base_mem_idx mr MemMM = Some memidx ->
+    f_locs f !! localimm lidx = Some (VAL_int32 ℓ32) ->
+    types_agree (translate_arep ι) v ->
+    ret = () /\
+    ⊢ ↪[frame] f -∗
+      ↪[RUN] -∗
+      ℓ ↦layout fs -∗
+      ℓ ↦heap ws -∗
+      memidxN ↦[wms][ℓ + byte_offset MemMM off]bits v -∗
+      ▷ value_interp rti sr se τ (SWords ws) -∗
+      ⌜path_offset fe τ π = Some off⌝ -∗
+      CWP es UNDER B; R {{ Φ }}.
+  Proof.
+    unfold load1.
+    intros Hcompile.
+    inv_cg_bind Hcompile [] ?wt ?wt ?wl ?wl es_get ?es_rest Hget Hcompile.
+    inv_cg_bind Hcompile [] ?wt ?wt ?wl ?wl es_ret ?es_rest Hret Hcompile.
+    cbn in Hret; inversion Hret; subst; clear Hret.
+    inv_cg_bind Hcompile [] ?wt ?wt ?wl ?wl es_load_w ?es_rest Hload_w Hcompile.
+    inv_cg_bind Hcompile [] ?wt ?wt ?wl ?wl es_wlalloc ?es_rest Hwlalloc Hcompile.
+    inv_cg_bind Hcompile [] ?wt ?wt ?wl ?wl es_save ?es_rest Hsave Hcompile.
+    subst.
+    apply wp_wlalloc in Hwlalloc.
+    destruct Hwlalloc as (Hidx & -> & -> & ->).
+    eapply wp_load_w in Hload_w.
+    destruct Hload_w as (_ & -> & -> & Hload_w).
+    inversion Hidx; subst n.
+    inv_cg_emit Hget; subst.
+    inv_cg_emit Hsave; subst.
+    clear Hretval Hretval0.
+    clear_nils.
+    destruct ret.
+    split; [reflexivity|].
+    iIntros "Hf Hrun Hfs Hws Hmem Hval %Hpath".
+    iApply (cwp_seq with "[Hf Hrun]").
+    {
+      iApply (cwp_local_get with "[] [$] [$]"); eauto.
+      now instantiate (1:= λ f' v', ⌜f' = f /\ v' = [VAL_int32 ℓ32]⌝%I).
+    }
+    iIntros (f' vs') "[-> ->] Hf Hrun".
+    rewrite app_assoc.
+    iApply (cwp_seq with "[Hf Hrun Hmem]").
+    {
+      iApply (Hload_w with "[$] [$] [$]").
+      1, 2, 3, 4: done.
+      iIntros "!> Hmem".
+      instantiate (1:= λ f' v', (⌜f' = f⌝ ∗ ⌜v' = [v]⌝ ∗ _)%I).
+      cbn.
+      iSplit; [done|].
+      iSplit; [done|].
+      iApply "Hmem".
+    }
+    iIntros (? ?) "(-> & -> & Hmem) Hf Hrun".
+    rewrite app_assoc.
+    set (vloc := localimm (W.Mk_localidx (fe_wlocal_offset fe + length wl))).
+    set (f' := {| f_locs := <[vloc := v]> (f_locs f);
+                  f_inst := f_inst f |}).
+    iApply (cwp_seq with "[Hf Hrun]").
+    {
+      iApply (cwp_local_tee with "[] [$] [$]").
+      - admit.
+      - now instantiate (1:= λ f'' v'', ⌜f'' = f' /\ v'' = [v]⌝%I).
+    }
+    iIntros (? ?) "(-> & ->) Hf Hrun".
+    unfold ite_gc_ptr in Hcompile.
+    admit.
+  Abort.
+
+  Lemma mem_load_copy_mm_spec se fe lidx off ιs wt wl ret wt' wl' es fs ws ℓ τ π ev B R :
+    run_codegen (memory.load mr fe MemMM Copy lidx off ιs) wt wl = inr (ret, wt', wl', es) ->
+    ret = () /\
+    ⊢ ℓ ↦layout fs -∗
+      ℓ ↦heap ws -∗
+      ▷ value_interp rti sr se τ (SWords ws) -∗
+      ⌜path_offset fe τ π = Some off⌝ -∗
+      CWP ev :: es UNDER B; R {{ fr'; vs', True }}.
+  Proof.
+  Abort.
+
+  Lemma cwp_mod2_test_1 f (idx: nat) k E :
+    ⊢ ⌜f.(f_locs) !! idx = Some (VAL_int32 (Wasm_int.Int32.repr k))⌝ →
+      ⌜((Wasm_int.Int32.unsigned (Wasm_int.Int32.repr k)) `mod` 2 = 0)%Z⌝ →
+      ↪[frame] f -∗
+      ↪[RUN] -∗
+      CWP [memory.W.BI_get_local idx;
+           memory.W.BI_const (memory.W.VAL_int32 (Wasm_int.int_of_Z i32m 1));
+           memory.W.BI_binop memory.W.T_i32 (memory.W.Binop_i memory.W.BOI_and);
+           memory.W.BI_testop memory.W.T_i32 memory.W.TO_eqz]
+          @ E
+          UNDER []; None
+          {{ f'; vs, ⌜f' = f /\ vs = [VAL_int32 (Wasm_int.Int32.repr 1)]⌝ }}.
+  Proof.
+    iIntros (Hidx Hmod) "Hf Hrun".
+    cwp_chomp 3%nat.
+    iApply (cwp_seq with "[Hf Hrun]").
+    - cwp_chomp 1%nat.
+      iApply (cwp_seq with "[Hf Hrun]").
+      + iApply (cwp_local_get with "[] [$] [$]"); first done.
+        instantiate (1 := λ f' vs, ⌜f' = f /\ vs = [VAL_int32 (Wasm_int.Int32.repr k)]⌝%I).
+        by iFrame.
+      + iIntros (w f' [-> ->]) "Hf Hrun".
+        iApply (cwp_binop with "[$] [$]").
+        * cbn.
+          reflexivity.
+        * instantiate (1 := λ f' vs, ⌜f' = f /\ vs = [VAL_int32 (Wasm_int.Int32.repr 0)]⌝%I).
+          cbn.
+          iPureIntro.
+          split; first done.
+          do 2 f_equal.
+          unfold Wasm_int.Int32.iand.
+          unfold Wasm_int.Int32.and.
+          f_equal.
+          rewrite (Z.land_ones _ 1); lias.
+    - iIntros (w f' [-> ->]) "Hf' Hrun".
+      iApply (cwp_testop_i32 with "[$] [$]").
+      + reflexivity.
+      + cbn.
+        iFrame.
+        iSplit; eauto.
+  Qed.
+
+  Lemma cwp_mod2_test_1_2 f (idx: nat) k E :
+    ⊢ ⌜f.(f_locs) !! idx = Some (VAL_int32 (Wasm_int.Int32.repr k))⌝ →
+    ⌜((Wasm_int.Int32.unsigned (Wasm_int.Int32.repr k)) `mod` 2 = 1)%Z⌝ →
+    ↪[frame] f -∗
+    ↪[RUN] -∗
+    CWP [memory.W.BI_get_local idx;
+         memory.W.BI_const (memory.W.VAL_int32 (Wasm_int.int_of_Z i32m 1));
+         memory.W.BI_binop memory.W.T_i32 (memory.W.Binop_i memory.W.BOI_and);
+         memory.W.BI_testop memory.W.T_i32 memory.W.TO_eqz]
+        @ E
+        UNDER []; None
+        {{ f'; vs, ⌜f' = f /\ vs = [VAL_int32 (Wasm_int.Int32.repr 0)]⌝ }}.
+  Proof.
+    iIntros (Hidx Hmod) "Hf Hrun".
+    cwp_chomp 3%nat.
+    iApply (cwp_seq with "[Hf Hrun]").
+    - cwp_chomp 1%nat.
+      iApply (cwp_seq with "[Hf Hrun]").
+      + iApply (cwp_local_get with "[] [$] [$]"); first done.
+        by instantiate (1 := λ f' vs, ⌜f' = f /\ vs = [VAL_int32 (Wasm_int.Int32.repr k)]⌝%I).
+      + iIntros (w f' [-> ->]) "Hf Hrun".
+        iApply (cwp_binop with "[$] [$]"); first done.
+        instantiate (1 := λ f' vs, ⌜f' = f /\ vs = [VAL_int32 (Wasm_int.Int32.repr 1)]⌝%I).
+        iPureIntro.
+        split; first done.
+        do 2 f_equal.
+        cbn.
+        unfold Wasm_int.Int32.iand.
+        unfold Wasm_int.Int32.and.
+        f_equal.
+        rewrite (Z.land_ones _ 1); lias.
+    - iIntros (w f' [-> ->]) "Hf' Hrun".
+      iApply (cwp_testop_i32 with "[$] [$]").
+      + reflexivity.
+      + cbn.
+        iFrame.
+        iSplit; eauto.
+  Qed.
+
+  Lemma cwp_mod4_sub3_test f (idx: nat) k E :
+    ⊢ ⌜f.(f_locs) !! idx = Some (VAL_int32 (Wasm_int.Int32.repr (k - 3)))⌝ →
+      ⌜((Wasm_int.Int32.unsigned (Wasm_int.Int32.repr k)) `mod` 4 = 0)%Z⌝ →
+      ↪[frame] f -∗
+      ↪[RUN] -∗
+      CWP [memory.W.BI_get_local idx;
+           memory.W.BI_const (memory.W.VAL_int32 (Wasm_int.int_of_Z i32m 2));
+           memory.W.BI_binop memory.W.T_i32 (memory.W.Binop_i memory.W.BOI_and);
+           memory.W.BI_testop memory.W.T_i32 memory.W.TO_eqz]
+          @ E
+          UNDER []; None
+          {{ f'; vs, ⌜f' = f /\ vs = [VAL_int32 (Wasm_int.Int32.repr 1)]⌝ }}.
+  Proof.
+    iIntros (Hidx Hmod) "Hf Hrun".
+    cwp_chomp 3%nat.
+    iApply (cwp_seq with "[Hf Hrun]").
+    - cwp_chomp 1%nat.
+      iApply (cwp_seq with "[Hf Hrun]").
+      + iApply (cwp_local_get with "[] [$] [$]"); first done.
+        by instantiate (1 := (λ f' vs, ⌜f' = f /\ vs = [VAL_int32 (Wasm_int.Int32.repr (k - 3))]⌝)%I).
+      + iIntros (w f' [-> ->]) "Hf Hrun".
+        iApply (cwp_binop with "[$] [$]").
+        * cbn.
+          reflexivity.
+        * iFrame.
+          instantiate (1 := (λ f' vs, ⌜f' = f /\ vs = [VAL_int32 (Wasm_int.Int32.repr 0)]⌝)%I).
+          iPureIntro.
+          split; first done.
+          cbn.
+          do 2 f_equal.
+          unfold Wasm_int.Int32.iand.
+          unfold Wasm_int.Int32.and.
+          f_equal.
+          unfold Wasm_int.Int32.repr, Wasm_int.Int32.unsigned in *; simpl in *.
+          rewrite Wasm_int.Int32.Z_mod_modulus_eq.
+          rewrite Wasm_int.Int32.Z_mod_modulus_eq in Hmod.
+          replace (Wasm_int.Int32.modulus) with (4 * 1073741824)%Z in Hmod; last done.
+          rewrite Z.mul_comm in Hmod.
+          rewrite Zaux.Zmod_mod_mult in Hmod; try done.
+          rewrite Zmod_divides in Hmod; last done.
+          destruct Hmod as [? ->].
+          unfold Wasm_int.Int32.modulus, Wasm_int.Int32.wordsize, Integers.Wordsize_32.wordsize, two_power_nat; simpl.
+          apply Z.bits_inj_iff.
+          intros i.
+          rewrite Z.land_spec.
+          rewrite Z.testbit_0_l.
+          destruct (Z.eq_dec i 1) as [-> | Hi].
+          ** apply andb_false_intro1.
+             replace (4294967296)%Z with (2 ^ 32)%Z; last lia.
+             rewrite Z.mod_pow2_bits_low; last lia.
+             replace (4)%Z with (2 ^ 2)%Z; last lia.
+             rewrite Z.mul_comm.
+             rewrite Z.add_bit1.
+             rewrite Z.mul_pow2_bits_low; last lia.
+             rewrite Z.mul_pow2_bits_low; last lia.
+             done.
+          ** rewrite (Z.pow2_bits_false 1 i); [|lia].
+             apply andb_false_r.
+    - iIntros (w f' [-> ->]) "Hf Hrun".
+      iApply (cwp_testop_i32 with "[$] [$]").
+      + reflexivity.
+      + cbn.
+        iFrame.
+        iSplit; eauto.
+  Qed.
+
+    Lemma cwp_mod4_sub1_test f (idx: nat) k E :
+    ⊢ ⌜f.(f_locs) !! idx = Some (VAL_int32 (Wasm_int.Int32.repr (k - 1)))⌝ →
+      ⌜((Wasm_int.Int32.unsigned (Wasm_int.Int32.repr k)) `mod` 4 = 0)%Z⌝ →
+      ↪[frame] f -∗
+      ↪[RUN] -∗
+      CWP [memory.W.BI_get_local idx;
+           memory.W.BI_const (memory.W.VAL_int32 (Wasm_int.int_of_Z i32m 2));
+           memory.W.BI_binop memory.W.T_i32 (memory.W.Binop_i memory.W.BOI_and);
+           memory.W.BI_testop memory.W.T_i32 memory.W.TO_eqz]
+          @ E
+          UNDER []; None
+          {{ f'; vs, ⌜f' = f⌝ ∗ ⌜vs = [VAL_int32 (Wasm_int.Int32.repr 0)]⌝ }}.
+  Proof.
+    iIntros (Hidx Hmod) "Hf Hrun".
+    cwp_chomp 3%nat.
+    iApply (cwp_seq with "[Hf Hrun]").
+    - cwp_chomp 1%nat.
+      iApply (cwp_seq with "[Hf Hrun]").
+      + iApply (cwp_local_get with "[] [$] [$]"); first done.
+        instantiate (1 := (λ f' vs, ⌜f' = f⌝ ∗ ⌜vs = [VAL_int32 (Wasm_int.Int32.repr (k - 1))]⌝)%I).
+        by iFrame.
+      + iIntros (w f' [-> ->]) "Hf Hrun".
+        iApply (cwp_binop with "[$] [$]").
+        * cbn.
+          reflexivity.
+        * iFrame.
+          instantiate (1 := (λ f' vs, ⌜f' = f⌝ ∗ ⌜vs = [VAL_int32 (Wasm_int.Int32.repr 2)]⌝)%I).
+          iPureIntro.
+          split; first done.
+          cbn.
+          do 2 f_equal.
+          unfold Wasm_int.Int32.iand.
+          unfold Wasm_int.Int32.and.
+          f_equal.
+          unfold Wasm_int.Int32.repr, Wasm_int.Int32.unsigned in *; simpl in *.
+          rewrite Wasm_int.Int32.Z_mod_modulus_eq.
+          rewrite Wasm_int.Int32.Z_mod_modulus_eq in Hmod.
+          replace (Wasm_int.Int32.modulus) with (4 * 1073741824)%Z in Hmod; last done.
+          rewrite Z.mul_comm in Hmod.
+          rewrite Zaux.Zmod_mod_mult in Hmod; try done.
+          rewrite Zmod_divides in Hmod; last done.
+          destruct Hmod as [? ->].
+          unfold Wasm_int.Int32.modulus, Wasm_int.Int32.wordsize, Integers.Wordsize_32.wordsize, two_power_nat; simpl.
+          apply Z.bits_inj_iff.
+          intros i.
+          rewrite Z.land_spec.
+          destruct (Z.eq_dec i 1) as [-> | Hi].
+          ** replace (4294967296)%Z with (2 ^ 32)%Z; last lia.
+             rewrite Z.mod_pow2_bits_low; last lia.
+             replace (4)%Z with (2 ^ 2)%Z; last lia.
+             rewrite Z.mul_comm.
+             rewrite Z.add_bit1.
+             rewrite Z.mul_pow2_bits_low; last lia.
+             rewrite Z.mul_pow2_bits_low; last lia.
+             done.
+          ** rewrite (Z.pow2_bits_false 1 i); [|lia].
+             apply andb_false_r.
+    - iIntros (w f' [-> ->]) "Hf Hrun".
+      iApply (cwp_testop_i32 with "[$] [$]").
+      + reflexivity.
+      + cbn.
+        iFrame.
+        iSplit; eauto.
+  Qed.
+
+  (* Note: The lemma assumes no input values to the case_ptr as no use case of it has needed it.
+     It should, however, be possible to prove a version  that assumes values on the stack. *)
+  Lemma cwp_case_ptr {A B} s E L R idx (c1 : codegen B) (c2: base_memory -> codegen A)
+    wt wt' wl wl' ts1 ts2 evs vs es x y z v (f: frame) Φ :
+    run_codegen (memory.case_ptr idx (Tf ts1 ts2) c1 c2) wt wl = inr (x, (y, z), wt', wl', es) ->
+    has_values evs vs ->
+    length ts1 = length vs ->
+    exists wt1 wt2 wt3 wl1 wl2 wl3 es1 es2 es3,
+      run_codegen c1 wt wl = inr (x, wt1, wl1, es1) /\
+      run_codegen (c2 MemMM) (wt ++ wt1) (wl ++ wl1) = inr (y, wt2, wl2, es2) /\
+      run_codegen (c2 MemGC) (wt ++ wt1 ++ wt2) (wl ++ wl1 ++ wl2) = inr (z, wt3, wl3, es3) /\
+      wt' = wt1 ++ wt2 ++ wt3 /\
+      wl' = wl1 ++ wl2 ++ wl3 /\
+      ⊢ ∀ ptr,
+        ↪[frame] f -∗
+        ↪[RUN] -∗
+        ⌜f.(f_locs) !! localimm idx = Some v⌝ -∗
+        atom_interp (PtrA ptr) v -∗
+        ▷ (↪[frame]f -∗
+            ↪[RUN] -∗
+            atom_interp (PtrA ptr) v -∗
+            match ptr with
+            | PtrInt z => CWP evs ++ es1 @ s; E UNDER []; R {{ Φ }}
+            | PtrHeap MemMM l => CWP evs ++ es2 @ s; E UNDER []; R {{ Φ }}
+            | PtrHeap MemGC l => CWP evs ++ es3 @ s; E UNDER []; R {{ Φ }}
+            end) -∗
+        CWP evs ++ es @ s; E UNDER L; R {{ Φ }}.
+  Proof.
+    intros Hcg Hevs Hlen.
+    assert (is_consts evs).
+    { eapply Is_true_true. eapply has_values_is_consts. by apply Is_true_true. }
+    assert (length evs = length ts1)
+      by (erewrite has_values_length; eauto).
+    unfold memory.case_ptr in Hcg.
+    inv_cg_bind Hcg [] ?wt ?wt ?wl ?wl ?es_isptr ?es_if_isptr Hcg_isptr Hcg_if_isptr.
+    inv_cg_emit_all Hcg_isptr.
+    subst.
+    rewrite -> !app_nil_l, !app_nil_r in *.
+    eapply (cwp_if_c s E) in Hcg_if_isptr; eauto.
+    destruct Hcg_if_isptr as (?wt & ?wt & ?wl & ?wl & es_int & es_case_m & Hcg_int & Hcg_case_m & -> & -> & Hwp_if_isptr).
+    inv_cg_bind Hcg_case_m [] ?wt ?wt ?wl ?wl ?es_mm_or_gc es_if_m Hcg_mm_or_gc Hcg_if_m.
+    inv_cg_emit_all Hcg_mm_or_gc.
+    subst.
+    eapply (cwp_if_c s E) in Hcg_if_m; eauto.
+    destruct Hcg_if_m as (?wt & ?wt & ?wl & ?wl & es_mm & es_gc & Hcg_mm & Hcg_gc & -> & -> & Hwp_if_m).
+    rewrite <- !app_assoc, !app_nil_r, !app_nil_l in *.
+    exists wt0, wt1, wt2, wl0, wl1, wl2.
+    exists es_int, es_mm, es_gc.
+    do 5 (split; first done).
+    clear Hcg_int Hcg_mm Hcg_gc Hretval Hretval0.
+    iIntros (ptr) "Hframe Hrun %Hlookup_f Hrep Hptr".
+    destruct ptr.
+    - iEval (cbn) in "Hrep".
+      iDestruct "Hrep" as "(%vn & -> & %rp & %Hrp & Hrep)".
+      destruct rp as [r|? ?].
+      + iPoseProof "Hrep" as "->".
+        inversion Hrp; subst.
+        rewrite app_assoc.
+        iApply (cwp_seq with "[Hframe Hrun]").
+        {
+          iApply cwp_val_app; eauto.
+          iApply cwp_label_take.
+          instantiate (2 := 0%nat).
+          iApply cwp_return_none.
+          iApply (cwp_wand with "[Hframe Hrun]").
+          {
+            iApply (cwp_mod2_test_1 with "[] [] [$] [$]"); eauto.
+            iPureIntro.
+            unfold Wasm_int.Int32.repr; simpl.
+            rewrite Wasm_int.Int32.Z_mod_modulus_eq.
+            unfold Wasm_int.Int32.modulus, Wasm_int.Int32.wordsize, Integers.Wordsize_32.wordsize.
+            unfold two_power_nat.
+            simpl.
+            apply mod32_mod2.
+          }
+          cbn.
+          instantiate (1:= λ f' vs', ⌜f' = f /\ vs' = vs ++ [VAL_int32 (Wasm_int.Int32.repr 1)]⌝%I).
+          iIntros (vs' f') "[-> ->]".
+          unfold fvs_combine; simpl; auto.
+        }
+        iIntros (vs' f') "[-> ->] Hf Hrun".
+        unfold to_consts; rewrite map_app -app_assoc.
+        erewrite <- has_values_to_consts_inv by eauto.
+        iApply (Hwp_if_isptr with "[$] [$]").
+        iLeft.
+        iSplit; [iPureIntro; done|].
+        iIntros "!> Hf Hrun".
+        iApply (cwp_label_wand with "[Hptr Hf Hrun]");
+          [| iApply label_ctx_wand_nil].
+        iApply ("Hptr" with "[$] [$]").
+        iExists _; eauto.
+      + done.
+    - iDestruct "Hrep" as "(%l & -> & %rp & %Hrep & Hroot)".
+      iPoseProof (root_pointer_heap_shp_inv with "Hroot") as "(%a & ->)".
+      inversion Hrep as [|? ? Hmod]; subst.
+      rewrite app_assoc.
+      iApply (cwp_seq with "[Hframe Hrun]").
+      {
+        iApply cwp_val_app; [eauto|].
+        iApply (cwp_wand with "[Hframe Hrun]").
+        {
+          iApply cwp_label_take.
+          instantiate (2 := 0%nat).
+          iApply cwp_return_none.
+          iApply (cwp_mod2_test_1_2 with "[] [] [$] [$]"); eauto.
+          unfold Wasm_int.Int32.repr; simpl.
+          rewrite Wasm_int.Int32.Z_mod_modulus_eq.
+          unfold Wasm_int.Int32.modulus, Wasm_int.Int32.wordsize, Integers.Wordsize_32.wordsize.
+          unfold two_power_nat.
+          simpl.
+          rewrite Z_mod_even_mod_2; last by rewrite <- Z.even_spec.
+          destruct μ; simpl.
+          1,2: apply N.Div0.mod_divides in Hmod as [c ->].
+          1,2: rewrite N2Z.inj_mul.
+          1,2: simpl.
+          1,2: rewrite Zmod_even.
+          1,2: rewrite Z.even_sub.
+          1,2: replace 4%Z with (2 * 2)%Z; last done.
+          1,2: rewrite <- Z.mul_assoc.
+          1,2: rewrite Z.even_even.
+          1,2: done.
+        }
+        unfold fvs_combine.
+        instantiate (1:= (λ f' vs', ⌜f' = f /\ vs' = vs ++ [VAL_int32 (Wasm_int.Int32.repr 0)]⌝ )%I).
+        by iIntros (f' v') "[-> ->]".
+      }
+      iIntros (w f' [-> ->]) "Hf Hrun".
+      unfold to_consts; rewrite map_app -app_assoc.
+      erewrite <- has_values_to_consts_inv by eauto.
+      iApply (Hwp_if_isptr with "[$] [$]").
+      iRight.
+      iSplit; first done.
+      iIntros "!> Hframe Hrun".
+      rewrite app_assoc.
+      destruct μ.
+      + iApply (cwp_seq with "[Hframe Hrun]").
+        {
+          iApply cwp_val_app; eauto.
+          iApply (cwp_wand with "[Hframe Hrun]").
+          {
+            simpl tag_address in Hlookup_f.
+            cbn.
+            rewrite <- (app_nil_l [_]).
+            rewrite app_nil_l.
+            iApply cwp_label_take.
+            instantiate (2 := 0%nat).
+            iApply cwp_return_none.
+            iApply (cwp_mod4_sub3_test with "[] [] [$] [$]"); eauto.
+            iPureIntro.
+            unfold Wasm_int.Int32.repr; simpl.
+            rewrite Wasm_int.Int32.Z_mod_modulus_eq.
+            unfold Wasm_int.Int32.modulus, Wasm_int.Int32.wordsize, Integers.Wordsize_32.wordsize.
+            unfold two_power_nat; simpl.
+            replace (4294967296)%Z with (4 * 1073741824)%Z; last done.
+            rewrite Z.mul_comm.
+            rewrite Zaux.Zmod_mod_mult; try done.
+            apply N2Z.inj_iff in Hmod.
+            rewrite N2Z.inj_mod in Hmod.
+            done.
+          }
+          iIntros (f' vs') "[-> ->]".
+          instantiate (1 := λ f' vs', ⌜f' = f /\ vs' = vs ++ [VAL_int32 (Wasm_int.Int32.repr 1)]⌝%I).
+          auto.
+        }
+        iIntros (w f' [-> ->]) "Hf Hrun".
+        unfold to_consts; rewrite map_app -app_assoc.
+        erewrite <- has_values_to_consts_inv by eauto.
+        iApply (Hwp_if_m with "[$] [$]").
+        iLeft.
+        iSplit; eauto.
+        iIntros  "!> Hf Hrun".
+        iApply (cwp_label_wand with "[Hptr Hroot Hf Hrun]");
+          [| iApply label_ctx_wand_nil].
+        iApply ("Hptr" with "[$] [$]").
+        iExists _; eauto.
+      + iApply (cwp_seq with "[Hframe Hrun]").
+        {
+          iApply cwp_val_app; eauto.
+          iApply (cwp_wand with "[Hframe Hrun]").
+          {
+            simpl tag_address in Hlookup_f.
+            cbn.
+            rewrite <- (app_nil_l [_]).
+            rewrite app_nil_l.
+            iApply cwp_label_take.
+            instantiate (2 := 0%nat).
+            iApply cwp_return_none.
+            iApply (cwp_mod4_sub1_test with "[//] [] [$] [$]").
+            iPureIntro.
+            unfold Wasm_int.Int32.repr; simpl.
+            rewrite Wasm_int.Int32.Z_mod_modulus_eq.
+            unfold Wasm_int.Int32.modulus, Wasm_int.Int32.wordsize, Integers.Wordsize_32.wordsize.
+            unfold two_power_nat; simpl.
+            replace (4294967296)%Z with (4 * 1073741824)%Z; last done.
+            rewrite Z.mul_comm.
+            rewrite Zaux.Zmod_mod_mult; try done.
+            apply N2Z.inj_iff in Hmod.
+            rewrite N2Z.inj_mod in Hmod.
+            done.
+          }
+          iIntros (f' vs') "[-> ->]".
+          instantiate (1 := λ f' vs', ⌜f' = f /\ vs' = vs ++ [VAL_int32 (Wasm_int.Int32.repr 0)]⌝%I).
+          auto.
+        }
+        iIntros (w f' [-> ->]) "Hf Hrun".
+        unfold to_consts; rewrite map_app -app_assoc.
+        erewrite <- has_values_to_consts_inv by eauto.
+        iApply (Hwp_if_m with "[$] [$]").
+        iRight.
+        iSplit; eauto.
+        iIntros  "!> Hf Hrun".
+        iApply (cwp_label_wand with "[Hptr Hroot Hf Hrun]");
+          [| iApply label_ctx_wand_nil].
+        iApply ("Hptr" with "[$] [$]").
+        iExists _; eauto.
+  Qed.
+
+  Lemma compat_load_copy M F L wt wt' wtf wl wl' wlf es' κ κser μ τ τval π pr :
+    let fe := fe_of_context F in
+    let WT := wt ++ wt' ++ wtf in
+    let WL := wl ++ wl' ++ wlf in
+    let ψ := InstrT [RefT κ μ τ] [RefT κ μ τ; τval] in
+    has_copyability F τval ExCopy ->
+    resolves_path τ π None pr ->
+    pr.(pr_target) = SerT κser τval ->
+    Forall (has_mono_size F) (pr_prefix pr) ->
+    has_instruction_type_ok F ψ L ->
+    run_codegen (compile_instr mr fe (ILoad ψ π Copy)) wt wl = inr ((), wt', wl', es') ->
+    ⊢ have_instr_type_sem rti sr mr M F L WT WL es' ψ L.
+  Proof.
+    intros fe WT WL ψ Hcopyability Hresolves Hser Hmonosize Htype Hcompile.
+    unfold WT, WL; clear WT WL. (* If the WT := or WL := become necessary, comment the unfold/clear*)
+    cbn in Hcompile.
+
+    (* Mechanically get through some of the first few things in compile_load *)
+    inv_cg_bind Hcompile off ?wt ?wt ?wl ?wl  es_fail ?es_rest Hoff Hcompile.
+    inv_cg_bind Hcompile ρ ?wt ?wt ?wl ?wl es_off ?es_rest Hρ Hcompile.
+    inv_cg_bind Hcompile ιs ?wt ?wt ?wl ?wl es_ρ ?es_rest Hιs Hcompile.
+    inv_cg_try_option Hρ; rename Heq_some into Hρ.
+    inv_cg_try_option Hιs; rename Heq_some into Hιs.
+    inv_cg_try_option Hoff; rename Heq_some into Hoff.
+    inv_cg_bind Hcompile a ?wt ?wt ?wl ?wl es_a ?es_rest Ha Hcompile.
+    cbn in Ha; inversion Ha; subst; clear Ha.
+    inv_cg_bind Hcompile res_emit ?wt ?wt ?wl ?wl  es_emit ?es_rest Hemit Hcompile.
+    inv_cg_emit Hemit.
+    inv_cg_bind Hcompile () ?wt ?wt ?wl ?wl es_empty ?es_rest Hempty Hcompile.
+    cbn in Hempty; inversion Hempty; subst; clear Hempty.
+    inv_cg_bind Hcompile [] ?wt ?wt ?wl ?wl  es_case_ptr ?es_rest Hcompile Hignore.
+    cbn in Hignore; inversion Hignore; subst; clear Hignore.
+
+    (* Some clean up *)
+    assert (Hu: u = ()). { by destruct u. }
+    assert (Hp: p = ((),())). { by destruct p as [[] []]. }
+    subst.
+    rewrite ?app_nil_r ?app_nil_l -?app_assoc.
+    rewrite ?app_nil_r ?app_nil_l -?app_assoc in Hcompile.
+    simpl app.
+    unfold have_instr_type_sem.
+    iIntros (se inst fr os vs evs θ B R Hse Hevs) "Hinst Hlbl Hret Hats Hvals Hfr Hrt Hf Hrun".
+    iEval (rewrite values_interp_one_eq; cbn) in "Hvals".
+    iPoseProof (value_interp_ref_sz with "Hvals") as "%Hlen_os".
+    iEval (rewrite value_interp_eq) in "Hvals".
+    iDestruct "Hvals" as (κ' Hκ') "[Harep Href]".
+    destruct κ'; [|done].
+    iDestruct "Harep" as "%Harep".
+    change instruction.W.T_i32 with T_i32 in *.
+    change prelude.W.Mk_localidx with Mk_localidx in *.
+    change instruction.W.BI_unreachable with BI_unreachable in *.
+    change instruction.W.BI_tee_local with BI_tee_local in *.
+    set (ptr_local := sum_list_with length (typing.fc_locals F) + length wl) in *.
+
+    cbn in Hκ'.
+    iAssert (⌜ptr_local < length (f_locs fr)⌝%I) as "%Hlen".
+    {
+      (* need a lemma about frame_interp, I think? *)
+      admit.
+    }
+    assert (Hκ: eval_rep se (AtomR PtrR) = Some l).
+    {
+      inversion Htype as [? ? ? Hmono Hctx]; subst.
+      destruct Hmono as [Hmono _].
+      rewrite Forall_singleton in Hmono.
+      inversion Hmono as [? ? ? Hrep Hismono]; subst.
+      inversion Hrep; subst.
+      apply rep_ref_kind_ptr in H; subst.
+      destruct H as [-> [χ' ->]].
+      unfold eval_kind in Hκ'.
+      apply bind_Some in Hκ'; destruct Hκ' as [l' [Heval Hret]].
+      inversion Hret; subst; auto.
+    }
+    cbn in Hκ; inversion Hκ; subst l.
+    destruct Harep as [os' [Hos Hareps]].
+    inversion Hos; subst os'; clear Hos.
+    iPoseProof (atoms_interp_length os vs with "Hats") as "%Hlen_os_vs".
+    pose proof (has_values_length _ _ Hevs) as Hlen_evs_vs.
+    destruct evs as [|ev [|ev' evs]]; try (cbn in *; congruence).
+    destruct vs as [|v [|v' vs]]; try (cbn in *; congruence).
+    destruct os as [|o [|o' os]]; try (cbn in *; congruence).
+    inversion Hareps as [| ? ? ? ? Harep _]; subst.
+    destruct o; inversion Harep; clear Harep Hareps.
+    cbn [app].
+    change (?x :: ?y :: ?z) with ([x; y] ++ z).
+    set (f' := {| f_locs := <[ptr_local:=v ]> (f_locs fr);
+                  f_inst := f_inst fr |}).
+    iApply (cwp_seq with "[Hf Hrun]").
+    {
+      change ([?ev; ?x]) with ([ev] ++ [x]).
+      rewrite (has_values_to_consts_inv _ _ Hevs).
+      iApply (cwp_local_tee with "[ ] [$] [$]"); eauto.
+      by instantiate (1:= λ f'' vs', ⌜f'' = f' /\ vs' = [v]⌝%I).
+    }
+    iIntros (f vs) "[-> ->] Hf Hrun".
+    eapply cwp_case_ptr in Hcompile.
+    2: do 2 instantiate (1 := []).
+    2, 3: done.
+    destruct Hcompile as (?wt & ?wt & ?wt & ?wl & ?wl & ?wl & ?es & ?es & ?es & Hcompile).
+    destruct Hcompile as (Hunr & Hload1 & Hload2 & Hwt0 & Hwl0 & Hspec).
+    rewrite atoms_interp_one_inv.
+    iDestruct "Hats" as "(%v' & %Hv' & Hat)".
+    inversion Hv'; subst v'; clear Hv'.
+    iApply cwp_val_app.
+    { instantiate (1 := [v]). apply Is_true_true. apply/andP; split => //. by apply/eqP. }
+    iApply (Hspec with "[$] [$] [] [$Hat]").
+    {
+      iPureIntro; cbn.
+      rewrite list_lookup_insert.
+      by rewrite decide_True.
+    }
+    iIntros "!> Hf Hrun Hat".
+    iEval (cbn) in "Href".
+    destruct μ as [|[|]]; first done.
+    - unfold ref_mm_interp.
+      iDestruct "Href" as (ℓ fs ws Hsv) "(Hℓl & Hℓh & Hws)".
+      inversion Hsv; subst.
+      rewrite value_interp_eq.
+      (* need lemma about memory.load *)
+      assert (Hlenιs: length ιs = 1) by admit.
+      destruct ιs as [| ι [| ? ? ]]; try discriminate Hlenιs.
+      cbn in Hload1.
+      admit.
+    - unfold ref_gc_interp.
+      iDestruct "Href" as (ℓ fs Hsv) "Hinv".
+      inversion Hsv; subst.
+      (* need lemma about memory.load *)
+      admit.
+  Admitted.
+
+End Fundamental.
