theories/iris/logrel/compat/ungroup.v
@@ -1,0 +1,48 @@
+Require Import RecordUpdate.RecordUpdate.
+From stdpp Require Import base list.
+
+From iris.proofmode Require Import base proofmode classes.
+
+From RichWasm.named_props Require Import named_props custom_syntax.
+From RichWasm.wasm Require Import operations.
+From RichWasm Require Import layout syntax typing.
+From RichWasm.compiler Require Import prelude codegen instruction module.
+From RichWasm.iris Require Import autowp memory util wp_codegen.
+From RichWasm.iris.language Require Import cwp logpred.
+From RichWasm.iris.logrel Require Import relations fundamental_kinding.
+
+Set Bullet Behavior "Strict Subproofs".
+Set Default Goal Selector "!".
+
+Section Fundamental.
+
+  Context `{!logrel_na_invs Σ}.
+  Context `{!wasmG Σ}.
+  Context `{!richwasmG Σ}.
+
+  Variable rti : rt_invariant Σ.
+  Variable sr : store_runtime.
+  Variable mr : module_runtime.
+
+  Lemma compat_ungroup M F L wt wt' wtf wl wl' wlf es' τs κ :
+    let fe := fe_of_context F in
+    let WT := wt ++ wt' ++ wtf in
+    let WL := wl ++ wl' ++ wlf in
+    let ψ := InstrT [ProdT κ τs] τs in
+    has_instruction_type_ok F ψ L ->
+    run_codegen (compile_instr mr fe (IUngroup ψ)) wt wl = inr ((), wt', wl', es') ->
+    ⊢ have_instr_type_sem rti sr mr M F L WT WL es' ψ L.
+  Proof.
+    (* intros fe WT WL ψ Hok Hcg. *)
+    (* inversion Hok as [F' ψ' L' Hmono Hok']. *)
+    (* subst F' ψ' L'. *)
+    (* cbn in Hcg; inversion Hcg; subst wt' wl' es'. *)
+    (* simpl to_e_list. *)
+    (* iApply sem_type_erased_nop; first done. *)
+    (* iIntros (se vs) "Hvs". *)
+    (* rewrite values_interp_one_eq value_interp_eq. *)
+    (* cbn. *)
+    (* iDestruct "Hvs" as "(%κ' & %Hκ' & Hkind & Hvs)". *)
+  Admitted.
+
+End Fundamental.
